Splinter/Journal/LinkedJournalRefinement.i.dfy
@@ -8,6 +8,7 @@ module LinkedJournalRefinement
 // TODO refines RefinementObligation(JournalLabels, PagedJournal)
 {
   import opened Options
+  import opened Maps
   import opened MsgHistoryMod
   import opened LSNMod
   import PagedJournal
@@ -52,6 +53,163 @@ module LinkedJournalRefinement
     RankedIPtrFraming(dv1, dv2, dv1.TheRanking(), dv2.TheRanking(), ptr);
   }
 
+  lemma RankedBuildTightShape(big: DiskView, root: Pointer, ranking: Ranking)
+    requires root.Some?
+    requires big.Decodable(root)
+    requires big.PointersRespectRank(ranking)
+    ensures
+      big.RankedBuildTight(big.entries[root.value].CroppedPrior(big.boundaryLSN), ranking) ==
+      DiskView(big.boundaryLSN, MapRemove1(big.RankedBuildTight(root, ranking).entries, root.value))
+  {
+    var next := big.entries[root.value].CroppedPrior(big.boundaryLSN);
+    if next.None? {
+      assert big.RankedBuildTight(big.entries[root.value].CroppedPrior(big.boundaryLSN), ranking) ==
+      DiskView(big.boundaryLSN, MapRemove1(big.RankedBuildTight(root, ranking).entries, root.value));
+    } else {
+      assert root.value !in big.RankedBuildTight(next, ranking).entries;
+      assert MapRemove1(big.RankedBuildTight(next, ranking).entries[root.value := big.entries[root.value]], root.value) == big.RankedBuildTight(next, ranking).entries;
+      calc {
+        big.RankedBuildTight(next, ranking);
+
+        var nextaddr := next.value;
+        DiskView(big.boundaryLSN, big.RankedBuildTight(big.entries[nextaddr].CroppedPrior(big.boundaryLSN), ranking).entries[nextaddr := big.entries[nextaddr]]);
+
+        var rootaddr := root.value;
+        var thing := big.RankedBuildTight(next, ranking).entries[rootaddr := big.entries[rootaddr]];
+        //assert thing == big.RankedBuildTight(root, ranking);
+        DiskView(big.boundaryLSN, MapRemove1(thing, rootaddr));
+
+        DiskView(big.boundaryLSN, MapRemove1(big.RankedBuildTight(root, ranking).entries, root.value));
+      }
+    }
+  }
+
+  lemma RankedIPtrIgnoresExtraBlocks(small: DiskView, ptr: Pointer, ranking: Ranking, big: DiskView)
+    requires small.WF()
+    requires big.WF()
+    requires small.IsNondanglingPointer(ptr)
+    requires big.PointersRespectRank(ranking)
+    requires small.IsSubDisk(big)
+    ensures big.RankedIPtr(ptr, ranking) == small.RankedIPtr(ptr, ranking)
+    decreases if ptr.Some? then ranking[ptr.value] else -1 // I can't believe this works, Rustan!
+  {
+    if ptr.Some? {
+      var next := big.entries[ptr.value].CroppedPrior(big.boundaryLSN);
+      RankedIPtrIgnoresExtraBlocks(small, next, ranking, big);
+    }
+  }
+
+  lemma TightSubDisk(big: DiskView, root: Pointer, ranking: Ranking, tight: DiskView)
+    requires big.Decodable(root)
+    requires big.PointersRespectRank(ranking)
+    requires tight == big.RankedBuildTight(root, ranking)
+    requires big.Acyclic()
+    requires tight.IsSubDisk(big);
+    ensures tight.IsTight(root)
+    decreases if root.Some? then ranking[root.value] else -1 // I can't believe this works, Rustan!
+  {
+    if root.Some? {
+      var next := big.entries[root.value].CroppedPrior(big.boundaryLSN);
+      var inner := big.RankedBuildTight(next, ranking);
+      RankedBuildTightShape(big, root, ranking);
+      TightSubDisk(big, next, ranking, inner);
+      assert inner.IsTight(next);
+      forall other:DiskView |
+          && other.Decodable(root)
+          && tight.IPtr(root) == other.IPtr(root)
+          && other.IsSubDisk(tight)
+          ensures other == tight {
+        var otherInner := DiskView(other.boundaryLSN, MapRemove1(other.entries, root.value));
+//        var otherInner := DiskView(other.boundaryLSN, map ki | ki in other.entries && ki != root.value :: other.entries[ki]);
+        assert otherInner.Decodable(next);
+//        if otherInner.IPtr(next) != inner.IPtr(next) {
+//          assert other.IPtr(root) != tight.IPtr(root);
+//          assert Some(PagedJournal.JournalRecord(jr.messageSeq, RankedIPtr(jr.CroppedPrior(boundaryLSN), ranking)))
+//        }
+        assert otherInner.IsSubDisk(inner);
+        RankedIPtrIgnoresExtraBlocks(otherInner, next, ranking, inner);
+        assert otherInner.RankedIPtr(next, ranking) == inner.RankedIPtr(next, ranking);
+        assert otherInner.PointersRespectRank(ranking);
+        assert inner.PointersRespectRank(ranking);
+        RankedIPtrFraming(otherInner, otherInner, ranking, otherInner.TheRanking(), next);
+        RankedIPtrFraming(inner, inner, ranking, inner.TheRanking(), next);
+        assert otherInner.RankedIPtr(next, otherInner.TheRanking()) == inner.RankedIPtr(next, inner.TheRanking());
+        assert otherInner.IPtr(next) == inner.IPtr(next);
+        assert otherInner == inner;
+        assert other == tight;
+      }
+      assert tight.IsTight(root);
+    }
+  }
+
+  lemma TightInterp(big: DiskView, root: Pointer, ranking: Ranking, tight: DiskView)
+    requires big.Decodable(root)
+    requires big.PointersRespectRank(ranking)
+    requires tight == big.RankedBuildTight(root, ranking)
+    requires big.Acyclic()
+    ensures tight.IsSubDisk(big)
+    ensures tight.IsTight(root)
+    ensures tight.Decodable(root)
+    ensures tight.IPtr(root) == big.IPtr(root)
+    ensures tight.Acyclic()
+    decreases if root.Some? then ranking[root.value] else -1 // I can't believe this works, Rustan!
+  {
+    if root.None? {
+      assert tight.IsSubDisk(big);
+      assert tight.IsTight(root);
+      assume false;
+      assert tight.Decodable(root);
+      assert tight.IPtr(root) == big.IPtr(root);
+      assert tight.Acyclic();
+    } else {
+      var next := big.entries[root.value].CroppedPrior(big.boundaryLSN);
+      var inner := big.RankedBuildTight(next, ranking);
+      TightInterp(big, next, ranking, inner);
+      assert tight.IsSubDisk(big);
+      forall other:DiskView |
+          && other.Decodable(root)
+          && tight.IPtr(root) == other.IPtr(root)
+          && other.IsSubDisk(tight)
+          ensures other == tight
+      {
+        forall k ensures k in tight.entries.Keys <==> k in other.entries.Keys {
+          if k in tight.entries.Keys {
+            if k == root.value {
+              assert k in other.entries.Keys;
+            } else {
+              assert k in inner.entries.Keys;
+              var otherInner := DiskView(other.boundaryLSN, map ki | ki in other.entries && ki != k :: other.entries[ki]);
+              assert otherInner.IsSubDisk(inner) by {
+                assert tight.entries.Keys == inner.entries.Keys + { root.value };
+                forall ko | ko in otherInner.entries ensures ko in inner.entries {
+                  assert ko != k;
+                  assert ko != root.value;
+                  assert ko in other.entries;
+                  assert ko in tight.entries;
+                  assert ko in inner.entries;
+                }
+              }
+              assert otherInner.Decodable(next);
+              assert otherInner.IPtr(root) == inner.IPtr(root);
+              assert otherInner == inner; // from inner.IsTight()
+              assert k in other.entries.Keys;
+            }
+          }
+          if k in other.entries.Keys {
+            assert k in tight.entries.Keys;
+          }
+        }
+        assert other.entries.Keys == tight.entries.Keys;
+        assert other == tight;
+      }
+      assert tight.IsTight(root);
+      assume false;
+      assert tight.Decodable(root);
+      assert tight.IPtr(root) == big.IPtr(root);
+      assert tight.Acyclic();
+    }
+  }
+
   //////////////////////////////////////////////////////////////////////////////
   // non-state-machine function & predicate refinement lemmas
 
@@ -85,6 +243,35 @@ module LinkedJournalRefinement
     if ptr.Some? && !(dv.entries[ptr.value].messageSeq.seqStart <= lsn) {
       DiscardInterp(dv, lsn, discarded, discarded.entries[ptr.value].CroppedPrior(discarded.boundaryLSN));
     }
+  }
+
+  lemma DiscardHarder(tj: TruncatedJournal, lsn: LSN, discarded: TruncatedJournal)
+    requires tj.WF()
+    requires tj.diskView.Acyclic()
+    requires tj.I().WF()
+    requires tj.I().I().CanDiscardTo(lsn)
+    requires tj.SeqStart() <= lsn
+    requires discarded == tj.DiscardOld(lsn)
+    ensures discarded.diskView.Acyclic();
+    ensures tj.I().WF();
+    ensures tj.I().DiscardOld(lsn) == discarded.I()
+  {
+    assert discarded.diskView.PointersRespectRank(tj.diskView.TheRanking());
+    DiscardInterp(tj.diskView, lsn, discarded.diskView, tj.freshestRec);
+//    if lsn < tj.SeqEnd() {
+//      assert discarded == TruncatedJournal(tj.freshestRec, tj.diskView.DiscardOld(lsn));
+//      assert discarded.I() == PagedJournal.TruncatedJournal(discarded.diskView.boundaryLSN, discarded.diskView.IPtr(tj.freshestRec));
+//      assert tj.I() == PagedJournal.TruncatedJournal(tj.diskView.boundaryLSN, tj.diskView.IPtr(tj.freshestRec));
+//      assert tj.I().DiscardOld(lsn) == PagedJournal.TruncatedJournal(lsn, PagedJournal.DiscardOldJournalRec(tj.I().freshestRec, lsn));
+//      assert discarded.diskView.boundaryLSN == lsn;
+//      assert discarded.diskView.IPtr(tj.freshestRec) == discarded.diskView.RankedIPtr(tj.freshestRec, discarded.diskView.TheRanking());
+//
+//      assert discarded.diskView.RankedIPtr(tj.freshestRec, discarded.diskView.TheRanking()) == PagedJournal.DiscardOldJournalRec(tj.diskView.IPtr(tj.freshestRec), lsn);
+//     
+//      assert discarded.diskView.RankedIPtr(tj.freshestRec, discarded.diskView.TheRanking()) == PagedJournal.DiscardOldJournalRec(tj.I().freshestRec, lsn);
+//      assert discarded.diskView.IPtr(tj.freshestRec) == PagedJournal.DiscardOldJournalRec(tj.I().freshestRec, lsn);
+//      assert tj.I().DiscardOld(lsn) == discarded.I();
+//    }
   }
     
   lemma SubDiskInterp(small: DiskView, big: DiskView, ptr: Pointer)
@@ -121,16 +308,39 @@ module LinkedJournalRefinement
       assert Inv(v');
     } else if step.DiscardOldStep? {
       var lsn := lbl.startLsn;
-      var croppedTJ := v.truncatedJournal.DiscardOld(lbl.startLsn);
-      var diskView := v.truncatedJournal.diskView;
+      var croppedTJ := v.truncatedJournal.DiscardOld(lsn);
+      var tightTJ := croppedTJ.BuildTight();
 
-      assert v'.truncatedJournal.diskView.PointersRespectRank(diskView.TheRanking());  // ranking witness gets across both DiscardOld and tightening
+      assert croppedTJ.diskView.PointersRespectRank(v.truncatedJournal.diskView.TheRanking());
+      assert croppedTJ.diskView.Acyclic();
+      TightInterp(croppedTJ.diskView, croppedTJ.freshestRec, croppedTJ.diskView.TheRanking(), tightTJ.diskView);
+      assert tightTJ.diskView.IsSubDisk(croppedTJ.diskView);
+      assert tightTJ.WF();
+      assert tightTJ.diskView.Acyclic();
+
+//      assert v'.truncatedJournal.diskView.PointersRespectRank(diskView.TheRanking());  // ranking witness gets across both DiscardOld and tightening
       if !(v.unmarshalledTail.seqStart <= lsn) {
         assert v.SeqStart() == v.truncatedJournal.I().I().seqStart by { v.truncatedJournal.I().BuildReceipt().TJFacts(); }
-        DiscardInterp(diskView, lsn, diskView.DiscardOld(lsn), v.truncatedJournal.freshestRec);
-        SubDiskInterp(v'.truncatedJournal.diskView, croppedTJ.diskView, croppedTJ.freshestRec);
+        DiscardInterp(croppedTJ.diskView, lsn, croppedTJ.diskView.DiscardOld(lsn), v.truncatedJournal.freshestRec);
+        SubDiskInterp(tightTJ.diskView, croppedTJ.diskView, croppedTJ.freshestRec);
+//        calc {
+//          v.truncatedJournal.I().DiscardOld(lsn).freshestRec;
+//          // original paged discard
+//          v.truncatedJournal.I().DiscardOldDefn(lsn).freshestRec;
+//
+//          croppedTJ.diskView.DiscardOld(lsn).RankedIPtr(v.truncatedJournal.freshestRec, croppedTJ.diskView.DiscardOld(lsn).TheRanking());
+//          PagedJournal.DiscardOldJournalRec(croppedTJ.diskView.IPtr(croppedTJ.freshestRec), lsn);
+//          croppedTJ.diskView.IPtr(croppedTJ.freshestRec);
+//        }
+//        calc {
+//          croppedTJ.I();
+//          PagedJournal.TruncatedJournal(croppedTJ.diskView.boundaryLSN, croppedTJ.diskView.IPtr(croppedTJ.freshestRec));
+//          v.truncatedJournal.I().DiscardOld(lsn);
+//        }
+        DiscardHarder(v.truncatedJournal, lsn, croppedTJ);
         assert croppedTJ.I() == v.truncatedJournal.I().DiscardOld(lsn); // Trigger for v'.I().WF()
       }
+      assert tightTJ.I() == croppedTJ.I();
       assert Inv(v');
     } else if step.InternalJournalMarshalStep? {
       // Witness new rank
@@ -180,6 +390,8 @@ module LinkedJournalRefinement
         }
         var croppedTJ := v.truncatedJournal.DiscardOld(lbl.startLsn);
         DiscardInterp(v.truncatedJournal.diskView, lsn, croppedTJ.diskView, v.truncatedJournal.freshestRec);
+        TightInterp(croppedTJ.diskView, croppedTJ.freshestRec, croppedTJ.diskView.TheRanking(), v'.truncatedJournal.diskView);
+        assert v'.truncatedJournal.diskView.IsSubDisk(croppedTJ.diskView);
         SubDiskInterp(v'.truncatedJournal.diskView, croppedTJ.diskView, croppedTJ.freshestRec);
       }
       assert PagedJournal.NextStep(I(v), I(v'), lbl.I(), PagedJournal.DiscardOldStep()); // witness step
@@ -190,5 +402,55 @@ module LinkedJournalRefinement
       assert false;
     }
   }
-}
 
+  // Exporting a utility for BlockCoordSystem to reason about the TruncatedJournal
+  // it takes away for inFlight.
+//  //////////////////////////////////////////////////////////////////////////////
+//  // Rob strategy
+//  predicate InFlightMemberOfEphemeral(eph: Variables, inFlight: TruncatedJournal)
+//  {
+//    && inFlight.diskView.IsSubDisk(eph.diskView)
+//    && eph.diskView.boundaryLSN <= inFlight.diskView.boundaryLSN
+//    && inFlight.freshestRec somewhere in eph.receipt
+//  }
+//
+//  lemma RobStyle(eph: Variables, inFlight: TruncatedJournal)
+//    requires InFlightMemberOfEphemeral(eph, inFlight)
+//    ensures inFlight.diskView.IsSubDisk(eph.DiscardOld(inFlight.SeqStart()).diskView)
+//
+//  lemma RobAdditionalOverwhelmingBurden(v: Variables, v': Variables, inFlight: TruncatedJournal)
+//    requires InFlightMemberOfEphemeral(v, inFlight)
+//    requires Next(v, v', anyLabel)
+//    ensures InFlightMemberOfEphemeral(v', inFlight)
+  //////////////////////////////////////////////////////////////////////////////
+
+  // This is a piece of an invariant that BlockCoordinationSystem maintains,
+  // not an invariant of the LinkedJournal.
+  predicate InFlightSubDiskProperty(v: Variables, inFlight: TruncatedJournal)
+  {
+    && v.WF()
+    && inFlight.WF()
+    && v.truncatedJournal.diskView.boundaryLSN <= inFlight.SeqStart()
+    && inFlight.diskView.IsSubDisk(v.truncatedJournal.DiscardOld(inFlight.SeqStart()).diskView)
+  }
+  
+  lemma InFlightSubDiskCreated(v: Variables, v': Variables, lbl: TransitionLabel)
+    requires lbl.FreezeForCommitLabel?
+    requires Next(v, v', lbl)
+    ensures InFlightSubDiskProperty(v', lbl.frozenJournal)
+  {
+    var cropped := v.truncatedJournal.DiscardOld(lbl.frozenJournal.SeqStart());
+    var tight := cropped.BuildTight();
+    TightInterp(cropped.diskView, cropped.freshestRec, cropped.diskView.TheRanking(), tight.diskView);
+  }
+
+  // TODO(jonh): Turns out this two lemma is entirely automated. Delete? Or export for automation control.
+  lemma InFlightSubDiskPreserved(v: Variables, v': Variables, inFlight: TruncatedJournal)
+    requires Next(v, v', InternalLabel())
+    requires InFlightSubDiskProperty(v, inFlight)
+    ensures InFlightSubDiskProperty(v', inFlight)
+  {
+  }
+  
+  //////////////////////////////////////////////////////////////////////////////
+}
